Fixed because of renamed definitions in Kraus_Families.

Limit_Process.thy
@@ -13,78 +13,78 @@ section \<open>Limit Processes\<close>
 text \<open>We need some concept of limes of kraus families, i.e.\ finite kraus maps tending to a 
 kraus map. Therefore, we define a filter on the Kraus family.\<close>
 
-text \<open>\<open>kraus_family_elems\<close> is the set of Kraus maps with only one element that are part of the 
+text \<open>\<open>kf_elems\<close> is the set of Kraus maps with only one element that are part of the 
 original Kraus map.\<close>
 
-lift_definition kraus_family_elems :: 
+lift_definition kf_elems :: 
 "('a::chilbert_space, 'b::chilbert_space, unit) kraus_family \<Rightarrow> ('a, 'b, unit) kraus_family set" is 
 "\<lambda>E. (\<lambda>x. {x}) ` E"
-by (auto simp add: kraus_family_finite)
+by (auto simp add: kf_finite)
 
-lemma kraus_family_elems_Rep_kraus_family:
-"kraus_family_elems \<EE> = (\<lambda>x. Abs_kraus_family {x}) ` Rep_kraus_family \<EE>"
-unfolding kraus_family_elems_def by auto
+lemma kf_elems_Rep_kraus_family:
+"kf_elems \<EE> = (\<lambda>x. Abs_kraus_family {x}) ` Rep_kraus_family \<EE>"
+unfolding kf_elems_def by auto
 
-lemma kraus_family_elems_finite:
-assumes "F \<in> kraus_family_elems \<EE>"
+lemma kf_elems_finite:
+assumes "F \<in> kf_elems \<EE>"
 shows "finite (Rep_kraus_family F)"
 using assms by transfer auto
 
-lemma kraus_family_bound_of_elems:
-assumes "F \<in> kraus_family_elems E" 
-shows "kraus_family_bound F \<le> kraus_family_bound E" 
+lemma kf_bound_of_elems:
+assumes "F \<in> kf_elems E" 
+shows "kf_bound F \<le> kf_bound E" 
 proof -
   have subset: "Rep_kraus_family F \<subseteq> Rep_kraus_family E" using assms by transfer auto
-  have "kraus_family_bound F = (\<Sum>(E, u)\<in>Rep_kraus_family F. E* o\<^sub>C\<^sub>L E)"
-    using assms kraus_family_bound_finite kraus_family_elems_finite by blast
-  also have "\<dots> \<le> kraus_family_bound E" using kraus_family_sums_bounded_by_bound[OF subset] by auto
+  have "kf_bound F = (\<Sum>(E, u)\<in>Rep_kraus_family F. E* o\<^sub>C\<^sub>L E)"
+    using assms kf_bound_finite kf_elems_finite by blast
+  also have "\<dots> \<le> kf_bound E" using kf_sums_bounded_by_bound[OF subset] by auto
   finally show ?thesis by linarith
 qed
 
-lemma kraus_family_elems_card_1:
-assumes "F \<in> kraus_family_elems E" 
+lemma kf_elems_card_1:
+assumes "F \<in> kf_elems E" 
 shows "card (Rep_kraus_family F) = 1"
 using assms by transfer auto
 
-lemma inj_on_kraus_family_singleton:
+lemma inj_on_kf_singleton:
 "inj_on (\<lambda>x. Abs_kraus_family {x}) (Rep_kraus_family \<EE>)" 
 by (metis (no_types, lifting) Abs_kraus_family_inverse finite.intros(1) finite.intros(2) 
-    inj_on_def kraus_family_finite mem_Collect_eq the_elem_eq)
+    inj_on_def kf_finite mem_Collect_eq the_elem_eq)
 
-lemma kraus_family_map_singleton:
-"(\<lambda>\<FF>. kraus_family_map \<FF> \<rho>) \<circ> (\<lambda>E. Abs_kraus_family {E::'a::chilbert_space \<Rightarrow>\<^sub>C\<^sub>L 'b::chilbert_space \<times> unit}) = 
+lemma kf_apply_singleton:
+"(\<lambda>\<FF>. kf_apply \<FF> \<rho>) \<circ> (\<lambda>E. Abs_kraus_family {E::'a::chilbert_space \<Rightarrow>\<^sub>C\<^sub>L 'b::chilbert_space \<times> unit}) = 
  (\<lambda>(E, _). sandwich_tc E \<rho>)"
 proof -
   have *: "eq_onp (\<lambda>x. x \<in> Collect kraus_family) {E} {E}" for E :: "'a \<Rightarrow>\<^sub>C\<^sub>L 'b \<times> unit" 
-    by (simp add: eq_onp_same_args kraus_family_finite)
-  then show ?thesis by (auto simp add: o_def kraus_family_map.abs_eq[OF *])
+    by (simp add: eq_onp_same_args kf_finite)
+  then show ?thesis by (auto simp add: o_def kf_apply.abs_eq[OF *])
 qed
 
-lemma kraus_family_map_singleton':
-"kraus_family_map (Abs_kraus_family {x}) \<rho> = sandwich_tc (fst x) \<rho>"
-by (simp add: Abs_kraus_family_inverse kraus_family_finite kraus_family_map.rep_eq)
+lemma kf_apply_singleton':
+"kf_apply (Abs_kraus_family {x}) \<rho> = sandwich_tc (fst x) \<rho>"
+by (simp add: Abs_kraus_family_inverse kf_finite kf_apply.rep_eq)
 
-lemma kraus_family_map_summable_on_kraus_family_elems:
+lemma kf_apply_summable_on_kf_elems:
 fixes \<EE> :: "('a::chilbert_space,'b::chilbert_space,unit) kraus_family"
-shows "(\<lambda>\<FF>. kraus_family_map \<FF> \<rho>) summable_on (kraus_family_elems \<EE>)"
-unfolding  kraus_family_elems_Rep_kraus_family 
-by (subst summable_on_reindex[OF inj_on_kraus_family_singleton], subst kraus_family_map_singleton, 
-    rule kraus_family_map_summable)
+shows "(\<lambda>\<FF>. kf_apply \<FF> \<rho>) summable_on (kf_elems \<EE>)"
+unfolding  kf_elems_Rep_kraus_family 
+by (subst summable_on_reindex[OF inj_on_kf_singleton], subst kf_apply_singleton, 
+    rule kf_map_summable)
 
-lemma kraus_family_map_has_sum_kraus_family_elems:
+lemma kf_apply_has_sum_kf_elems:
 fixes \<EE> :: "('a::chilbert_space,'b::chilbert_space,unit) kraus_family"
-shows "((\<lambda>\<FF>. kraus_family_map \<FF> \<rho>) has_sum (kraus_family_map \<EE> \<rho>)) (kraus_family_elems \<EE>)"
-unfolding  kraus_family_elems_Rep_kraus_family 
-by (subst has_sum_reindex[OF inj_on_kraus_family_singleton], subst kraus_family_map_singleton, 
-    simp add: kraus_family_map_has_sum)
+shows "((\<lambda>\<FF>. kf_apply \<FF> \<rho>) has_sum (kf_apply \<EE> \<rho>)) (kf_elems \<EE>)"
+unfolding  kf_elems_Rep_kraus_family 
+by (subst has_sum_reindex[OF inj_on_kf_singleton], subst kf_apply_singleton, 
+    simp add: kf_map_has_sum)
 
-lemma kraus_family_map_abs_summable_on_kraus_family_elems:
+lemma kf_apply_abs_summable_on_kf_elems:
 fixes \<EE> :: "('a::chilbert_space,'b::chilbert_space,unit) kraus_family"
-shows "(\<lambda>\<FF>. kraus_family_map \<FF> \<rho>) abs_summable_on (kraus_family_elems \<EE>)"
-unfolding kraus_family_elems_Rep_kraus_family
-apply (subst abs_summable_on_reindex[OF inj_on_kraus_family_singleton], 
-       subst kraus_family_map_singleton)
-using Rep_kraus_family kraus_family_map_abs_summable by blast
+shows "(\<lambda>\<FF>. kf_apply \<FF> \<rho>) abs_summable_on (kf_elems \<EE>)"
+unfolding kf_elems_Rep_kraus_family
+apply (subst abs_summable_on_reindex[OF inj_on_kf_singleton], 
+       subst kf_apply_singleton)
+using Rep_kraus_family kf_map_abs_summable by blast
 
 
 
@@ -93,21 +93,21 @@ A sub-adversary is then defined as a sequence of $n$ elements of the respective 
 Adding all sub-adversaries together yields the original Kraus map.\<close>
 
 definition finite_kraus_subadv :: "'a kraus_adv \<Rightarrow> nat \<Rightarrow> 'a kraus_adv set" where
-"finite_kraus_subadv \<EE> n =  PiE {0..<n+1} (\<lambda>i. kraus_family_elems (\<EE> i))"
+"finite_kraus_subadv \<EE> n =  PiE {0..<n+1} (\<lambda>i. kf_elems (\<EE> i))"
 
 lemma finite_kraus_subadv_I:
 assumes "f \<in> finite_kraus_subadv \<EE> n" "i<n+1"
-shows "f i \<in> kraus_family_elems (\<EE> i)"
+shows "f i \<in> kf_elems (\<EE> i)"
 using assms unfolding finite_kraus_subadv_def by auto
 
 
 lemma finite_kraus_subadv_rewrite:
 "finite_kraus_subadv \<EE> (Suc n) = 
-  (\<lambda>(x,f). fun_upd f (Suc n) x) ` (kraus_family_elems (\<EE> (Suc n)) \<times> finite_kraus_subadv \<EE> n)"
+  (\<lambda>(x,f). fun_upd f (Suc n) x) ` (kf_elems (\<EE> (Suc n)) \<times> finite_kraus_subadv \<EE> n)"
 by (metis PiE_insert_eq Suc_eq_plus1 finite_kraus_subadv_def set_upt_Suc)
 
 lemma finite_kraus_subadv_rewrite_inj:
-"inj_on (\<lambda>(x, f). f(Suc n := x)) (kraus_family_elems (\<EE> (Suc n)) \<times> finite_kraus_subadv \<EE> n)"
+"inj_on (\<lambda>(x, f). f(Suc n := x)) (kf_elems (\<EE> (Suc n)) \<times> finite_kraus_subadv \<EE> n)"
 unfolding inj_on_def proof (safe, goal_cases)
   case (1 a b aa ba) then show ?case by (metis fun_upd_eqD)
 next
@@ -121,17 +121,17 @@ next
 qed 
 
 
-lemma norm_kraus_family_map_singleton_trace_tc:
+lemma norm_kf_apply_singleton_trace_tc:
 assumes "0 \<le> \<rho>"
-shows "norm (kraus_family_map (Abs_kraus_family {x}) \<rho>) = trace_tc (sandwich_tc (fst x) \<rho>)"
-by (subst norm_tc_pos, intro kraus_family_map_pos[OF assms], subst kraus_family_map_singleton') auto
+shows "norm (kf_apply (Abs_kraus_family {x}) \<rho>) = trace_tc (sandwich_tc (fst x) \<rho>)"
+by (subst norm_tc_pos, intro kf_apply_pos[OF assms], subst kf_apply_singleton') auto
  
 
-lemma infsum_norm_kraus_family_map_step:
+lemma infsum_norm_kf_apply_step:
 assumes \<rho>n_summable: "\<rho>n summable_on finite_kraus_subadv \<EE> n"
 and pos: "\<And>x. x \<in> finite_kraus_subadv \<EE> n \<Longrightarrow> 0 \<le> \<rho>n x"
-shows "(\<lambda>x. \<Sum>\<^sub>\<infinity>y\<in>finite_kraus_subadv \<EE> n. norm (kraus_family_map x (\<rho>n y))) 
-    abs_summable_on kraus_family_elems (\<EE> (Suc n))"
+shows "(\<lambda>x. \<Sum>\<^sub>\<infinity>y\<in>finite_kraus_subadv \<EE> n. norm (kf_apply x (\<rho>n y))) 
+    abs_summable_on kf_elems (\<EE> (Suc n))"
 proof -
   define \<rho> where "\<rho> = infsum \<rho>n (finite_kraus_subadv \<EE> n)"
   have "((\<lambda>y. trace_tc (sandwich_tc E y)) o (\<lambda>y. \<rho>n y) has_sum trace_tc (sandwich_tc E \<rho>))
@@ -144,10 +144,10 @@ proof -
     by (intro infsumI) (auto simp add: o_def \<rho>_def)
 
   let ?f1 = "(\<lambda>(E,x). \<bar>\<Sum>\<^sub>\<infinity>y\<in>finite_kraus_subadv \<EE> n. trace_tc (sandwich_tc E (\<rho>n y))\<bar>)"
-  let ?f2 = "(\<lambda>x. \<bar>\<Sum>\<^sub>\<infinity>y\<in>finite_kraus_subadv \<EE> n. norm (kraus_family_map (Abs_kraus_family {x}) (\<rho>n y))\<bar>)"
+  let ?f2 = "(\<lambda>x. \<bar>\<Sum>\<^sub>\<infinity>y\<in>finite_kraus_subadv \<EE> n. norm (kf_apply (Abs_kraus_family {x}) (\<rho>n y))\<bar>)"
 
   have "(\<lambda>(E, x). sandwich_tc E \<rho>) abs_summable_on Rep_kraus_family (\<EE> (Suc n))"
-    using Rep_kraus_family kraus_family_map_abs_summable by blast
+    using Rep_kraus_family kf_map_abs_summable by blast
   then have f1_summable: "?f1 summable_on Rep_kraus_family (\<EE> (Suc n))" 
     unfolding sandwich_tc_lim \<rho>_def[symmetric] using trace_tc_abs_summable_on o_def
     by (metis (mono_tags, lifting) abs_summable_summable norm_abs split_def summable_on_cong)  
@@ -157,9 +157,9 @@ proof -
     proof (subst summable_on_cong[of "Rep_kraus_family (\<EE> (Suc n))" ?f1 ?f2], goal_cases)
       case (1 x)
       have infsum: "(\<Sum>\<^sub>\<infinity>y\<in>finite_kraus_subadv \<EE> n. trace_tc (sandwich_tc (fst x) (\<rho>n y))) = 
-        (\<Sum>\<^sub>\<infinity>y\<in>finite_kraus_subadv \<EE> n. norm (kraus_family_map (Abs_kraus_family {x}) (\<rho>n y)))"
+        (\<Sum>\<^sub>\<infinity>y\<in>finite_kraus_subadv \<EE> n. norm (kf_apply (Abs_kraus_family {x}) (\<rho>n y)))"
       by (subst infsum_of_real[symmetric], intro infsum_cong, 
-          subst norm_kraus_family_map_singleton_trace_tc)
+          subst norm_kf_apply_singleton_trace_tc)
          (use pos in \<open>auto\<close>)
       then show ?case by (auto simp add: split_def abs_complex_def)
     next
@@ -168,9 +168,9 @@ proof -
     qed 
     then show ?thesis using f1_summable by auto
   qed
-  then show ?thesis unfolding  kraus_family_elems_Rep_kraus_family 
-    by (subst summable_on_reindex[OF inj_on_kraus_family_singleton]) 
-       (use kraus_family_map_singleton in \<open>auto simp add: o_def\<close> )
+  then show ?thesis unfolding  kf_elems_Rep_kraus_family 
+    by (subst summable_on_reindex[OF inj_on_kf_singleton]) 
+       (use kf_apply_singleton in \<open>auto simp add: o_def\<close> )
 qed
 
 
@@ -191,20 +191,20 @@ fixes \<EE> :: "'a kraus_adv"
 shows "(\<lambda>f. run_mixed_adv n f UB init X Y H) abs_summable_on (finite_kraus_subadv \<EE> n)"
 proof (induct n)
   case 0
-  have "inj_on (\<lambda>f. f 0) (\<Pi>\<^sub>E i\<in>{0}. kraus_family_elems (\<EE> i))" 
+  have "inj_on (\<lambda>f. f 0) (\<Pi>\<^sub>E i\<in>{0}. kf_elems (\<EE> i))" 
     unfolding  PiE_over_singleton_iff inj_on_def by auto
   then have inj: "inj_on (\<lambda>f. f 0) (finite_kraus_subadv \<EE> 0)" 
     unfolding finite_kraus_subadv_def by simp
-  have "(\<lambda>\<FF>. kraus_family_map \<FF> (tc_selfbutter init)) abs_summable_on
-     (kraus_family_elems (\<EE> 0))" using kraus_family_map_abs_summable_on_kraus_family_elems by auto
+  have "(\<lambda>\<FF>. kf_apply \<FF> (tc_selfbutter init)) abs_summable_on
+     (kf_elems (\<EE> 0))" using kf_apply_abs_summable_on_kf_elems by auto
   moreover {
-    have "x \<in> kraus_family_elems (\<EE> 0) \<Longrightarrow>
-         x \<in> (\<lambda>x. x 0) ` (\<Pi>\<^sub>E i\<in>{0}. kraus_family_elems (\<EE> i))" for x
+    have "x \<in> kf_elems (\<EE> 0) \<Longrightarrow>
+         x \<in> (\<lambda>x. x 0) ` (\<Pi>\<^sub>E i\<in>{0}. kf_elems (\<EE> i))" for x
       unfolding PiE_over_singleton_iff by (simp add: image_iff)
-    then have "(\<lambda>f. f 0) ` finite_kraus_subadv \<EE> 0 = kraus_family_elems (\<EE> 0)" 
+    then have "(\<lambda>f. f 0) ` finite_kraus_subadv \<EE> 0 = kf_elems (\<EE> 0)" 
      by (auto simp add: finite_kraus_subadv_I finite_kraus_subadv_def)     
   }
-  ultimately have "(\<lambda>\<FF>. kraus_family_map \<FF> (tc_selfbutter init)) o (\<lambda>f. f 0) abs_summable_on (finite_kraus_subadv \<EE> 0)" 
+  ultimately have "(\<lambda>\<FF>. kf_apply \<FF> (tc_selfbutter init)) o (\<lambda>f. f 0) abs_summable_on (finite_kraus_subadv \<EE> 0)" 
    by (subst abs_summable_on_reindex[OF inj, symmetric]) auto
   then show ?case by auto
 next
@@ -217,25 +217,25 @@ next
     "(\<lambda>f. \<rho>n f) abs_summable_on finite_kraus_subadv \<EE> n"
     unfolding \<rho>n_def using sandwich_tc_abs_summable_on[OF Suc] by (auto simp add: o_def)
 
-  have one: "(\<lambda>xa. kraus_family_map x (\<rho>n (xa(Suc n := x)))) abs_summable_on finite_kraus_subadv \<EE> n" 
-    if "x \<in> kraus_family_elems (\<EE> (Suc n))" for x
-    using \<rho>n_Suc_indiff \<rho>n_abs_summable_on finite_kraus_family_map_abs_summable_on by fastforce
+  have one: "(\<lambda>xa. kf_apply x (\<rho>n (xa(Suc n := x)))) abs_summable_on finite_kraus_subadv \<EE> n" 
+    if "x \<in> kf_elems (\<EE> (Suc n))" for x
+    using \<rho>n_Suc_indiff \<rho>n_abs_summable_on finite_kf_apply_abs_summable_on by fastforce
 
   have \<rho>n_summable: "\<rho>n summable_on finite_kraus_subadv \<EE> n" 
     using Suc \<rho>n_def \<rho>n_abs_summable_on abs_summable_summable by blast
   have pos: "x \<in> finite_kraus_subadv \<EE> n \<Longrightarrow> 0 \<le> \<rho>n x" for x
     by (simp add: \<rho>n_def run_mixed_adv_pos sandwich_tc_pos)
-  have two: "(\<lambda>x. \<Sum>\<^sub>\<infinity>y\<in>finite_kraus_subadv \<EE> n. norm (kraus_family_map x (\<rho>n (y(Suc n := x))))) 
-    abs_summable_on kraus_family_elems (\<EE> (Suc n))" 
-  unfolding \<rho>n_Suc_indiff by (rule infsum_norm_kraus_family_map_step[OF \<rho>n_summable pos])
+  have two: "(\<lambda>x. \<Sum>\<^sub>\<infinity>y\<in>finite_kraus_subadv \<EE> n. norm (kf_apply x (\<rho>n (y(Suc n := x))))) 
+    abs_summable_on kf_elems (\<EE> (Suc n))" 
+  unfolding \<rho>n_Suc_indiff by (rule infsum_norm_kf_apply_step[OF \<rho>n_summable pos])
 
-  have lim: "(\<lambda>x. kraus_family_map (x (Suc n)) (\<rho>n x)) abs_summable_on finite_kraus_subadv \<EE> (Suc n)"
+  have lim: "(\<lambda>x. kf_apply (x (Suc n)) (\<rho>n x)) abs_summable_on finite_kraus_subadv \<EE> (Suc n)"
   apply (subst finite_kraus_subadv_rewrite)
   apply (subst abs_summable_on_reindex[OF finite_kraus_subadv_rewrite_inj])
   apply (unfold o_def case_prod_beta) 
   apply (subst abs_summable_on_Sigma_iff)
   using one two by auto
-  then have "(\<lambda>f. kraus_family_map (f (Suc n)) (sandwich_tc ((X;Y) (Uquery H) o\<^sub>C\<^sub>L UB n)
+  then have "(\<lambda>f. kf_apply (f (Suc n)) (sandwich_tc ((X;Y) (Uquery H) o\<^sub>C\<^sub>L UB n)
    (run_mixed_adv n f UB init X Y H))) abs_summable_on
    (finite_kraus_subadv \<EE> (Suc n))" 
   unfolding \<rho>n_def[symmetric] by auto
@@ -254,24 +254,24 @@ shows "((\<lambda>f. run_mixed_adv n f UB init X Y H) has_sum run_mixed_adv n \<
   (finite_kraus_subadv \<EE> n)"
 proof (induct n)
   case 0
-  have "inj_on (\<lambda>f. f 0) (\<Pi>\<^sub>E i\<in>{0}. kraus_family_elems (\<EE> i))" 
+  have "inj_on (\<lambda>f. f 0) (\<Pi>\<^sub>E i\<in>{0}. kf_elems (\<EE> i))" 
     unfolding  PiE_over_singleton_iff inj_on_def by auto
   then have inj: "inj_on (\<lambda>f. f 0) (finite_kraus_subadv \<EE> 0)" 
     unfolding finite_kraus_subadv_def by simp
-  have rew: "(\<lambda>f. kraus_family_map (f 0) (tc_selfbutter init)) = 
-    (\<lambda>\<FF>. kraus_family_map \<FF> (tc_selfbutter init)) o (\<lambda>f. f 0)" by auto
-  have "((\<lambda>\<FF>. kraus_family_map \<FF> (tc_selfbutter init)) has_sum 
-     kraus_family_map (\<EE> 0) (tc_selfbutter init))
-     (kraus_family_elems (\<EE> 0))" using kraus_family_map_has_sum_kraus_family_elems by auto
+  have rew: "(\<lambda>f. kf_apply (f 0) (tc_selfbutter init)) = 
+    (\<lambda>\<FF>. kf_apply \<FF> (tc_selfbutter init)) o (\<lambda>f. f 0)" by auto
+  have "((\<lambda>\<FF>. kf_apply \<FF> (tc_selfbutter init)) has_sum 
+     kf_apply (\<EE> 0) (tc_selfbutter init))
+     (kf_elems (\<EE> 0))" using kf_apply_has_sum_kf_elems by auto
   moreover {
-    have "x \<in> kraus_family_elems (\<EE> 0) \<Longrightarrow>
-         x \<in> (\<lambda>x. x 0) ` (\<Pi>\<^sub>E i\<in>{0}. kraus_family_elems (\<EE> i))" for x
+    have "x \<in> kf_elems (\<EE> 0) \<Longrightarrow>
+         x \<in> (\<lambda>x. x 0) ` (\<Pi>\<^sub>E i\<in>{0}. kf_elems (\<EE> i))" for x
       unfolding PiE_over_singleton_iff by (simp add: image_iff)
-    then have "(\<lambda>f. f 0) ` finite_kraus_subadv \<EE> 0 = kraus_family_elems (\<EE> 0)" 
+    then have "(\<lambda>f. f 0) ` finite_kraus_subadv \<EE> 0 = kf_elems (\<EE> 0)" 
      by (auto simp add: finite_kraus_subadv_I finite_kraus_subadv_def)     
   }
-  ultimately have "((\<lambda>f. kraus_family_map (f 0) (tc_selfbutter init)) has_sum
-     kraus_family_map (\<EE> 0) (tc_selfbutter init)) (finite_kraus_subadv \<EE> 0)" 
+  ultimately have "((\<lambda>f. kf_apply (f 0) (tc_selfbutter init)) has_sum
+     kf_apply (\<EE> 0) (tc_selfbutter init)) (finite_kraus_subadv \<EE> 0)" 
   unfolding rew by (subst has_sum_reindex[OF inj, symmetric]) auto
   then show ?case by auto
 next
@@ -295,42 +295,42 @@ next
       unfolding \<rho>n_def by (metis (no_types) run_mixed_adv_abs_summable)
   qed
 
-  have one: "((\<lambda>y. kraus_family_map x (\<rho>n (y(Suc n := x)))) has_sum kraus_family_map x \<rho>)
-          (finite_kraus_subadv \<EE> n)" if "x \<in> kraus_family_elems (\<EE> (Suc n))" for x
+  have one: "((\<lambda>y. kf_apply x (\<rho>n (y(Suc n := x)))) has_sum kf_apply x \<rho>)
+          (finite_kraus_subadv \<EE> n)" if "x \<in> kf_elems (\<EE> (Suc n))" for x
     unfolding \<rho>n_Suc_indiff by (smt (verit, best) \<rho>n_has_sum_\<rho> comp_eq_dest_lhs 
-      finite_kraus_family_map_has_sum has_sum_cong)
-  have two: "((\<lambda>x. kraus_family_map x \<rho>) has_sum kraus_family_map (\<EE> (Suc n)) \<rho>)
-     (kraus_family_elems (\<EE> (Suc n)))" 
-     by (simp add: kraus_family_map_has_sum_kraus_family_elems)
+      finite_kf_apply_has_sum has_sum_cong)
+  have two: "((\<lambda>x. kf_apply x \<rho>) has_sum kf_apply (\<EE> (Suc n)) \<rho>)
+     (kf_elems (\<EE> (Suc n)))" 
+     by (simp add: kf_apply_has_sum_kf_elems)
 
-  have "(\<lambda>(x,f). kraus_family_map x (\<rho>n (f(Suc n := x)))) abs_summable_on
-    kraus_family_elems (\<EE> (Suc n)) \<times> finite_kraus_subadv \<EE> n"
+  have "(\<lambda>(x,f). kf_apply x (\<rho>n (f(Suc n := x)))) abs_summable_on
+    kf_elems (\<EE> (Suc n)) \<times> finite_kraus_subadv \<EE> n"
   proof (unfold \<rho>n_Suc_indiff, subst abs_summable_on_Sigma_iff, safe, goal_cases)
     case (1 x)
-    then show ?case using \<rho>n_abs_summable_on finite_kraus_family_map_abs_summable_on by auto
+    then show ?case using \<rho>n_abs_summable_on finite_kf_apply_abs_summable_on by auto
   next
     case 2
     then show ?case 
-      by (intro infsum_norm_kraus_family_map_step[OF abs_summable_summable[OF \<rho>n_abs_summable_on]]) 
+      by (intro infsum_norm_kf_apply_step[OF abs_summable_summable[OF \<rho>n_abs_summable_on]]) 
          (auto simp add: \<rho>n_def run_mixed_adv_pos sandwich_tc_pos)
   qed
-  then have "(\<lambda>(x,f). kraus_family_map x (\<rho>n (f(Suc n := x)))) summable_on
-    kraus_family_elems (\<EE> (Suc n)) \<times> finite_kraus_subadv \<EE> n"
+  then have "(\<lambda>(x,f). kf_apply x (\<rho>n (f(Suc n := x)))) summable_on
+    kf_elems (\<EE> (Suc n)) \<times> finite_kraus_subadv \<EE> n"
   using abs_summable_summable by blast
-  then have three: "(\<lambda>x. kraus_family_map (fst x) (\<rho>n ((snd x)(Suc n := fst x)))) summable_on
-    kraus_family_elems (\<EE> (Suc n)) \<times> finite_kraus_subadv \<EE> n"
+  then have three: "(\<lambda>x. kf_apply (fst x) (\<rho>n ((snd x)(Suc n := fst x)))) summable_on
+    kf_elems (\<EE> (Suc n)) \<times> finite_kraus_subadv \<EE> n"
     by (metis (no_types, lifting) split_def summable_on_cong)
 
   have lim: 
-    "((\<lambda>f. kraus_family_map (f (Suc n)) (\<rho>n f)) has_sum kraus_family_map (\<EE> (Suc n)) \<rho>)
+    "((\<lambda>f. kf_apply (f (Suc n)) (\<rho>n f)) has_sum kf_apply (\<EE> (Suc n)) \<rho>)
      (finite_kraus_subadv \<EE> (Suc n))" 
   apply (subst finite_kraus_subadv_rewrite)
   apply (subst has_sum_reindex[OF finite_kraus_subadv_rewrite_inj])
   apply (unfold o_def case_prod_beta) 
-  apply (intro has_sum_SigmaI[where g = "(\<lambda>x. kraus_family_map x \<rho>)"]) 
+  apply (intro has_sum_SigmaI[where g = "(\<lambda>x. kf_apply x \<rho>)"]) 
   by (auto simp add: one two three)
-  then have "((\<lambda>f. kraus_family_map (f (Suc n)) (sandwich_tc ((X;Y) (Uquery H) o\<^sub>C\<^sub>L UB n)
-   (run_mixed_adv n f UB init X Y H))) has_sum kraus_family_map (\<EE> (Suc n))
+  then have "((\<lambda>f. kf_apply (f (Suc n)) (sandwich_tc ((X;Y) (Uquery H) o\<^sub>C\<^sub>L UB n)
+   (run_mixed_adv n f UB init X Y H))) has_sum kf_apply (\<EE> (Suc n))
    (sandwich_tc ((X;Y) (Uquery H) o\<^sub>C\<^sub>L UB n) (run_mixed_adv n \<EE> UB init X Y H)))
    (finite_kraus_subadv \<EE> (Suc n))" 
   unfolding \<rho>n_def \<rho>_def by auto
@@ -350,96 +350,96 @@ unfolding run_mixed_A_def by (rule run_mixed_adv_has_sum)
 
 lemma run_mixed_B_has_sum:
 "((\<lambda>f. run_mixed_adv d f (US S) init_B X_for_B Y_for_B H) has_sum run_mixed_B kraus_B H S) 
-  (finite_kraus_subadv (\<lambda>n. kraus_family_Fst (kraus_B n)) d)"
+  (finite_kraus_subadv (\<lambda>n. kf_Fst (kraus_B n)) d)"
 unfolding run_mixed_B_def by (rule run_mixed_adv_has_sum)
 
 
 lemma run_mixed_B_count_has_sum:
 "((\<lambda>f. run_mixed_adv d f (\<lambda>_. U_S' S) init_B_count X_for_C Y_for_C H) has_sum run_mixed_B_count kraus_B H S) 
-  (finite_kraus_subadv (\<lambda>n. kraus_family_Fst (kraus_B n)) d)"
+  (finite_kraus_subadv (\<lambda>n. kf_Fst (kraus_B n)) d)"
 unfolding run_mixed_B_count_def by (rule run_mixed_adv_has_sum)
 
 
-lemma kraus_family_elems_kraus_family_Fst:
-"kraus_family_elems (kraus_family_Fst \<EE>) = (\<lambda>f. kraus_family_Fst f) ` kraus_family_elems \<EE>"
+lemma kf_elems_kf_Fst:
+"kf_elems (kf_Fst \<EE>) = (\<lambda>f. kf_Fst f) ` kf_elems \<EE>"
 by transfer auto
 
 
 
 lemma finite_kraus_subadv_Fst_invert:
-"finite_kraus_subadv (\<lambda>m.  (kraus_family_Fst :: _\<Rightarrow>(('a \<times> 'c) ell2,_,_) kraus_family) (\<EE> m)) n =  
- (\<lambda>f. \<lambda>i\<in>{0..<n+1}. kraus_family_Fst (f i)) ` (finite_kraus_subadv \<EE> n)"
-unfolding finite_kraus_subadv_def kraus_family_elems_kraus_family_Fst
+"finite_kraus_subadv (\<lambda>m.  (kf_Fst :: _\<Rightarrow>(('a \<times> 'c) ell2,_,_) kraus_family) (\<EE> m)) n =  
+ (\<lambda>f. \<lambda>i\<in>{0..<n+1}. kf_Fst (f i)) ` (finite_kraus_subadv \<EE> n)"
+unfolding finite_kraus_subadv_def kf_elems_kf_Fst
 proof (induct n)
   case 0
-  have " (\<Pi>\<^sub>E i\<in>{0..<0 + 1}. kraus_family_Fst ` kraus_family_elems (\<EE> i)) =  
-    (\<Pi>\<^sub>E i\<in>{0}. kraus_family_Fst ` kraus_family_elems (\<EE> i))" by auto
-  also have "\<dots> = (\<Union>b\<in>kraus_family_elems (\<EE> 0). {\<lambda>x\<in>{0}. kraus_family_Fst b})" 
+  have " (\<Pi>\<^sub>E i\<in>{0..<0 + 1}. kf_Fst ` kf_elems (\<EE> i)) =  
+    (\<Pi>\<^sub>E i\<in>{0}. kf_Fst ` kf_elems (\<EE> i))" by auto
+  also have "\<dots> = (\<Union>b\<in>kf_elems (\<EE> 0). {\<lambda>x\<in>{0}. kf_Fst b})" 
     unfolding PiE_over_singleton_iff by auto
-  also have "\<dots> = (\<Union>b\<in>kraus_family_elems (\<EE> 0). (\<lambda>f. \<lambda>i\<in>{0}. kraus_family_Fst (f i)) ` {\<lambda>x\<in>{0}. b})"
+  also have "\<dots> = (\<Union>b\<in>kf_elems (\<EE> 0). (\<lambda>f. \<lambda>i\<in>{0}. kf_Fst (f i)) ` {\<lambda>x\<in>{0}. b})"
   proof -
-    have "(\<lambda>x\<in>{0}. kraus_family_Fst b) = (\<lambda>a\<in>{0}. kraus_family_Fst (if a = 0 then b else undefined))" for b
+    have "(\<lambda>x\<in>{0}. kf_Fst b) = (\<lambda>a\<in>{0}. kf_Fst (if a = 0 then b else undefined))" for b
       by fastforce
     then show ?thesis  by (intro Union_cong) auto
   qed
-  also have "\<dots> = (\<lambda>f. \<lambda>i\<in>{0}. kraus_family_Fst (f i)) `(\<Union>b\<in>kraus_family_elems (\<EE> 0). {\<lambda>x\<in>{0}. b})"
+  also have "\<dots> = (\<lambda>f. \<lambda>i\<in>{0}. kf_Fst (f i)) `(\<Union>b\<in>kf_elems (\<EE> 0). {\<lambda>x\<in>{0}. b})"
     unfolding image_UN by auto
-  also have "\<dots> = (\<lambda>f. \<lambda>i\<in>{0..<0+1}. kraus_family_Fst (f i)) ` (\<Pi>\<^sub>E i\<in>{0}. kraus_family_elems (\<EE> i))" 
+  also have "\<dots> = (\<lambda>f. \<lambda>i\<in>{0..<0+1}. kf_Fst (f i)) ` (\<Pi>\<^sub>E i\<in>{0}. kf_elems (\<EE> i))" 
     unfolding PiE_over_singleton_iff by auto
-  also have "\<dots> = (\<lambda>f. \<lambda>i\<in>{0..<0+1}. kraus_family_Fst (f i)) ` (\<Pi>\<^sub>E i\<in>{0..<0+1}. kraus_family_elems (\<EE> i))" 
+  also have "\<dots> = (\<lambda>f. \<lambda>i\<in>{0..<0+1}. kf_Fst (f i)) ` (\<Pi>\<^sub>E i\<in>{0..<0+1}. kf_elems (\<EE> i))" 
     by auto
   finally show ?case by blast
 next
   case (Suc n)
-  let ?prodset = "kraus_family_elems (\<EE> (Suc n)) \<times>(\<Pi>\<^sub>E i\<in>{0..<n+1}. kraus_family_elems (\<EE> i))"
-  have "(\<Pi>\<^sub>E i\<in>{0..<Suc n + 1}. (kraus_family_Fst :: _\<Rightarrow>(('a \<times> 'c) ell2,_,_) kraus_family) ` 
-    kraus_family_elems (\<EE> i)) =  
-    (\<Pi>\<^sub>E i\<in>(insert (Suc n) {0..<Suc n}). kraus_family_Fst ` kraus_family_elems (\<EE> i))" 
+  let ?prodset = "kf_elems (\<EE> (Suc n)) \<times>(\<Pi>\<^sub>E i\<in>{0..<n+1}. kf_elems (\<EE> i))"
+  have "(\<Pi>\<^sub>E i\<in>{0..<Suc n + 1}. (kf_Fst :: _\<Rightarrow>(('a \<times> 'c) ell2,_,_) kraus_family) ` 
+    kf_elems (\<EE> i)) =  
+    (\<Pi>\<^sub>E i\<in>(insert (Suc n) {0..<Suc n}). kf_Fst ` kf_elems (\<EE> i))" 
     by (auto simp add: set_upt_Suc)
-  also have "\<dots> = (\<lambda>(y, g). g(Suc n := y)) ` (kraus_family_Fst ` kraus_family_elems (\<EE> (Suc n)) \<times>
-     (\<Pi>\<^sub>E i\<in>{0..<n+1}. kraus_family_Fst ` kraus_family_elems (\<EE> i)))" 
+  also have "\<dots> = (\<lambda>(y, g). g(Suc n := y)) ` (kf_Fst ` kf_elems (\<EE> (Suc n)) \<times>
+     (\<Pi>\<^sub>E i\<in>{0..<n+1}. kf_Fst ` kf_elems (\<EE> i)))" 
     by (subst PiE_insert_eq) auto
-  also have "\<dots> = (\<lambda>(y, g). g(Suc n := y)) ` (kraus_family_Fst ` kraus_family_elems (\<EE> (Suc n)) \<times>
-     ((\<lambda>f. \<lambda>i\<in>{0..<n+1}. kraus_family_Fst (f i)) ` (\<Pi>\<^sub>E i\<in>{0..<n+1}. kraus_family_elems (\<EE> i))))" 
+  also have "\<dots> = (\<lambda>(y, g). g(Suc n := y)) ` (kf_Fst ` kf_elems (\<EE> (Suc n)) \<times>
+     ((\<lambda>f. \<lambda>i\<in>{0..<n+1}. kf_Fst (f i)) ` (\<Pi>\<^sub>E i\<in>{0..<n+1}. kf_elems (\<EE> i))))" 
     by (subst Suc) auto
   also have "\<dots> = (\<lambda>(y, g). g(Suc n := y)) ` 
-    (\<lambda>(a,x). (kraus_family_Fst a, restrict (\<lambda>i. kraus_family_Fst (x i)) {0..<n+1})) ` ?prodset" 
+    (\<lambda>(a,x). (kf_Fst a, restrict (\<lambda>i. kf_Fst (x i)) {0..<n+1})) ` ?prodset" 
     by (simp add: image_paired_Times)
-  also have "\<dots> = (\<lambda>(y, g). (restrict (\<lambda>i. kraus_family_Fst (g i)) {0..<n+1})
-    (Suc n := kraus_family_Fst y)) ` ?prodset"
+  also have "\<dots> = (\<lambda>(y, g). (restrict (\<lambda>i. kf_Fst (g i)) {0..<n+1})
+    (Suc n := kf_Fst y)) ` ?prodset"
     by (subst image_image) (simp add: split_def) 
-  also have "\<dots> = (\<lambda>(y, g). restrict ((\<lambda>i. kraus_family_Fst (g i))(Suc n := kraus_family_Fst y))
+  also have "\<dots> = (\<lambda>(y, g). restrict ((\<lambda>i. kf_Fst (g i))(Suc n := kf_Fst y))
     (insert (Suc n) {0..<n+1})) ` ?prodset"
     by (subst restrict_upd) auto
-  also have "\<dots> = (\<lambda>(y, g). restrict ((\<lambda>i. kraus_family_Fst (g i))(Suc n := kraus_family_Fst y))
+  also have "\<dots> = (\<lambda>(y, g). restrict ((\<lambda>i. kf_Fst (g i))(Suc n := kf_Fst y))
     {0..<Suc n + 1}) ` ?prodset" using semiring_norm(174) set_upt_Suc by presburger
-  also have "\<dots> = (\<lambda>(y, g). restrict (\<lambda>i. kraus_family_Fst ((g(Suc n:=y)) i))
+  also have "\<dots> = (\<lambda>(y, g). restrict (\<lambda>i. kf_Fst ((g(Suc n:=y)) i))
     {0..<Suc n + 1}) ` ?prodset" 
   proof -
-    have rew: "(\<lambda>i. kraus_family_Fst (g i))(Suc n := kraus_family_Fst y) = 
-      (\<lambda>i. (kraus_family_Fst :: _\<Rightarrow>(('a \<times> 'c) ell2,_,_) kraus_family) ((g(Suc n:=y)) i))" for g y 
+    have rew: "(\<lambda>i. kf_Fst (g i))(Suc n := kf_Fst y) = 
+      (\<lambda>i. (kf_Fst :: _\<Rightarrow>(('a \<times> 'c) ell2,_,_) kraus_family) ((g(Suc n:=y)) i))" for g y 
       by fastforce
     show ?thesis by (subst rew) auto
   qed
-  also have "\<dots> = (\<lambda>f. restrict (\<lambda>i. kraus_family_Fst (f i)) {0..<Suc n + 1}) ` 
+  also have "\<dots> = (\<lambda>f. restrict (\<lambda>i. kf_Fst (f i)) {0..<Suc n + 1}) ` 
     (\<lambda>(a,g). g(Suc n:= a)) ` ?prodset" 
     by (smt (verit, best) image_cong image_image restrict_ext split_def)
-  also have "\<dots> = (\<lambda>f. restrict (\<lambda>i. kraus_family_Fst (f i)) {0..<Suc n + 1}) ` 
-    (\<Pi>\<^sub>E i\<in>(insert (Suc n) {0..<Suc n}). kraus_family_elems (\<EE> i))" 
+  also have "\<dots> = (\<lambda>f. restrict (\<lambda>i. kf_Fst (f i)) {0..<Suc n + 1}) ` 
+    (\<Pi>\<^sub>E i\<in>(insert (Suc n) {0..<Suc n}). kf_elems (\<EE> i))" 
     by (metis Suc_eq_plus1 finite_kraus_subadv_def finite_kraus_subadv_rewrite set_upt_Suc)
-  also have "\<dots> = (\<lambda>f. \<lambda>i\<in>{0..<Suc n + 1}. kraus_family_Fst (f i)) ` 
-    (\<Pi>\<^sub>E i\<in>{0..<Suc n+1}. kraus_family_elems (\<EE> i))" by (simp add: set_upt_Suc)
+  also have "\<dots> = (\<lambda>f. \<lambda>i\<in>{0..<Suc n + 1}. kf_Fst (f i)) ` 
+    (\<Pi>\<^sub>E i\<in>{0..<Suc n+1}. kf_elems (\<EE> i))" by (simp add: set_upt_Suc)
   finally show ?case by blast
 qed
 
 
 
-lemma inj_on_kraus_family_Fst:
-"inj_on (\<lambda>f. \<lambda>n\<in>{0..<n+1}. (kraus_family_Fst (f n) :: (('a \<times> 'b) ell2, _, _) kraus_family)) 
+lemma inj_on_kf_Fst:
+"inj_on (\<lambda>f. \<lambda>n\<in>{0..<n+1}. (kf_Fst (f n) :: (('a \<times> 'b) ell2, _, _) kraus_family)) 
   (finite_kraus_subadv \<EE> n)"
 unfolding inj_on_def proof (safe, goal_cases)
   case (1 x y)
-  have eq: "(kraus_family_Fst (x i) :: (('a \<times> 'b) ell2, ('a \<times> 'b) ell2, _) kraus_family) = kraus_family_Fst (y i)"
+  have eq: "(kf_Fst (x i) :: (('a \<times> 'b) ell2, ('a \<times> 'b) ell2, _) kraus_family) = kf_Fst (y i)"
     if "i<Suc n" for i using fun_cong[of _ _ i, OF 1(3)] that by auto
   have "x i = y i" if "i<Suc n" for i using eq[OF that] proof (transfer, safe, goal_cases)
     case (1 x i y a)
@@ -470,16 +470,16 @@ unfolding inj_on_def proof (safe, goal_cases)
 qed
 
 
-lemma run_mixed_adv_kraus_family_Fst_restricted:
-"run_mixed_adv m (\<lambda>n. kraus_family_Fst (f n)) U init' X' Y' H =
- run_mixed_adv m (\<lambda>n\<in>{0..<m + 1}. kraus_family_Fst (f n)) U init' X' Y' H"
+lemma run_mixed_adv_kf_Fst_restricted:
+"run_mixed_adv m (\<lambda>n. kf_Fst (f n)) U init' X' Y' H =
+ run_mixed_adv m (\<lambda>n\<in>{0..<m + 1}. kf_Fst (f n)) U init' X' Y' H"
 proof (induct m arbitrary: f)
   case (Suc m)
-  let ?f1 = "(\<lambda>a. if a < Suc m then (kraus_family_Fst ::_\<Rightarrow>(('a \<times> 'b) ell2,_,_) kraus_family) (f a) 
+  let ?f1 = "(\<lambda>a. if a < Suc m then (kf_Fst ::_\<Rightarrow>(('a \<times> 'b) ell2,_,_) kraus_family) (f a) 
     else undefined)"
-  let ?f2 = "(\<lambda>a. if a < Suc (Suc m) then (kraus_family_Fst ::_\<Rightarrow>(('a \<times> 'b) ell2,_,_) kraus_family) (f a) 
+  let ?f2 = "(\<lambda>a. if a < Suc (Suc m) then (kf_Fst ::_\<Rightarrow>(('a \<times> 'b) ell2,_,_) kraus_family) (f a) 
     else undefined)"
-  have f12: "?f1(Suc m:= kraus_family_Fst (f (Suc m))) = ?f2" by fastforce
+  have f12: "?f1(Suc m:= kf_Fst (f (Suc m))) = ?f2" by fastforce
   have eq: "run_mixed_adv m ?f1 U init' X' Y' H = 
             run_mixed_adv m ?f2 U init' X' Y' H"
     unfolding f12[symmetric] by (subst run_mixed_adv_Suc_indifferent) auto
@@ -491,11 +491,11 @@ lemma run_mixed_B_has_sum':
 "((\<lambda>f. run_mixed_B f H S) has_sum run_mixed_B kraus_B H S) (finite_kraus_subadv kraus_B d)"
   (is "(?f has_sum ?x) ?A") 
 proof -
-  have inj: "inj_on (\<lambda>f. \<lambda>n\<in>{0..<d + 1}. kraus_family_Fst (f n)) (finite_kraus_subadv kraus_B d)" 
-    using inj_on_kraus_family_Fst by auto
+  have inj: "inj_on (\<lambda>f. \<lambda>n\<in>{0..<d + 1}. kf_Fst (f n)) (finite_kraus_subadv kraus_B d)" 
+    using inj_on_kf_Fst by auto
   have rew: "?f = (\<lambda>f. run_mixed_adv d f (US S) init_B X_for_B Y_for_B H) o 
-    (\<lambda>f. \<lambda>n\<in>{0..<d + 1}. kraus_family_Fst (f n))" unfolding run_mixed_B_def
-  using run_mixed_adv_kraus_family_Fst_restricted[where init' = init_B and X' = X_for_B and Y'=Y_for_B] 
+    (\<lambda>f. \<lambda>n\<in>{0..<d + 1}. kf_Fst (f n))" unfolding run_mixed_B_def
+  using run_mixed_adv_kf_Fst_restricted[where init' = init_B and X' = X_for_B and Y'=Y_for_B] 
   by auto
   show ?thesis unfolding rew  by (subst has_sum_reindex[OF inj, symmetric]) 
     (unfold finite_kraus_subadv_Fst_invert[symmetric], rule run_mixed_B_has_sum)
@@ -507,11 +507,11 @@ lemma run_mixed_B_count_has_sum':
 "((\<lambda>f. run_mixed_B_count f H S) has_sum run_mixed_B_count kraus_B H S) (finite_kraus_subadv kraus_B d)"
   (is "(?f has_sum ?x) ?A") 
 proof -
-  have inj: "inj_on (\<lambda>f. \<lambda>n\<in>{0..<d + 1}. kraus_family_Fst (f n)) (finite_kraus_subadv kraus_B d)" 
-    using inj_on_kraus_family_Fst by auto
+  have inj: "inj_on (\<lambda>f. \<lambda>n\<in>{0..<d + 1}. kf_Fst (f n)) (finite_kraus_subadv kraus_B d)" 
+    using inj_on_kf_Fst by auto
   have rew: "?f = (\<lambda>f. run_mixed_adv d f (\<lambda>_. U_S' S) init_B_count X_for_C Y_for_C H) o 
-    (\<lambda>f. \<lambda>n\<in>{0..<d + 1}. kraus_family_Fst (f n))" unfolding run_mixed_B_count_def
-  using run_mixed_adv_kraus_family_Fst_restricted[where init' = init_B_count and X' = X_for_C and Y'=Y_for_C]  
+    (\<lambda>f. \<lambda>n\<in>{0..<d + 1}. kf_Fst (f n))" unfolding run_mixed_B_count_def
+  using run_mixed_adv_kf_Fst_restricted[where init' = init_B_count and X' = X_for_C and Y'=Y_for_C]  
     by auto
   show ?thesis unfolding rew  by (subst has_sum_reindex[OF inj, symmetric]) 
     (unfold finite_kraus_subadv_Fst_invert[symmetric], rule run_mixed_B_count_has_sum)
@@ -541,17 +541,17 @@ qed
 lemma fin_subadv_fin_Rep_kraus_family:
 assumes "F \<in> finite_kraus_subadv E n" "i < n+1" "n<d+1"
 shows "finite (Rep_kraus_family (F i))"
-using assms unfolding finite_kraus_subadv_def using kraus_family_elems_finite by fastforce
+using assms unfolding finite_kraus_subadv_def using kf_elems_finite by fastforce
 
 lemma fin_subadv_bound_leq_id:
 assumes "F \<in> finite_kraus_subadv E d" 
 assumes "i < d+1"
-assumes E_norm_id: "\<And>i. i < d+1 \<Longrightarrow> kraus_family_bound (E i) \<le> id_cblinfun"
-shows "kraus_family_bound (F i) \<le> id_cblinfun"
+assumes E_norm_id: "\<And>i. i < d+1 \<Longrightarrow> kf_bound (E i) \<le> id_cblinfun"
+shows "kf_bound (F i) \<le> id_cblinfun"
 proof -
-  have "F i \<in> kraus_family_elems (E i)" using assms unfolding finite_kraus_subadv_def by auto
-  then have "kraus_family_bound (F i) \<le> kraus_family_bound (E i)" 
-    using kraus_family_bound_of_elems by auto
+  have "F i \<in> kf_elems (E i)" using assms unfolding finite_kraus_subadv_def by auto
+  then have "kf_bound (F i) \<le> kf_bound (E i)" 
+    using kf_bound_of_elems by auto
   then show ?thesis using E_norm_id[OF assms(2)] by auto
 qed
 
@@ -560,8 +560,8 @@ lemma fin_subadv_nonzero:
 assumes "F \<in> finite_kraus_subadv E n" "i < n+1" "n<d+1"
 shows "Rep_kraus_family (F i) \<noteq> {}"
 proof -
-  have "F i \<in> kraus_family_elems (E i)" using assms unfolding finite_kraus_subadv_def by auto
-  then show ?thesis using kraus_family_elems_card_1 by fastforce
+  have "F i \<in> kf_elems (E i)" using assms unfolding finite_kraus_subadv_def by auto
+  then show ?thesis using kf_elems_card_1 by fastforce
 qed
 
 end
